trunk/examples/Arrays/regression/MultipleStores.bpl
@@ -10,16 +10,22 @@ var a : [int]int;
 var i : int;
 var tmp : int;
 var tmp2 : int;
+var tmp3 : int;
+var tmp4 : int;
 
 
 procedure main() returns ()
-modifies a, tmp, tmp2;
+modifies a, tmp, tmp2, tmp3, tmp4;
 {
   a[i] := 1;
   tmp := a[i];
   a[i] := 2;
   tmp2 := a[i];
   a[i] := 5;
+  tmp3 := a[i];
+  a[i] := 10;
+  tmp4 := a[i];
+  a[i] := 20;
   assert tmp!=tmp2;
   assert tmp!=a[i];
   assert a[i]!=tmp2;
